Add global read/write lock to semantics

src/CCLPrimitives.v
@@ -14,12 +14,28 @@ Section Primitives.
 
   Ltac begin_prim :=
     unfold cprog_spec, cprog_ok; simpl; intros;
-    repeat deex.
+    repeat deex;
+    try match goal with
+        | [ H: context[let (n, m) := ?a in _] |- _ ] =>
+          let n := fresh n in
+          let m := fresh m in
+          destruct a as [m n];
+          simpl in *;
+          Automation.safe_intuition
+        end.
+
+  Ltac inv_opt :=
+    match goal with
+    | [ H: Some _ = Some _ |- _ ] =>
+      inversion H; subst; clear H
+    end.
 
   Theorem BeginRead_ok : forall tid a,
       cprog_spec G tid
                  (fun v '(sigma_i, sigma) =>
-                    {| precondition := Sigma.disk sigma a = Some (v, NoReader);
+                    {| precondition :=
+                         Sigma.disk sigma a = Some (v, NoReader) /\
+                         Sigma.l sigma = WriteLock;
                        postcondition :=
                          fun '(sigma_i', sigma') _ =>
                            sigma_i' = sigma_i /\
@@ -28,18 +44,18 @@ Section Primitives.
   Proof.
     begin_prim.
     inv_bind; inv_exec.
+    inv_opt.
 
     eapply H2; eauto; simpl.
     intuition eauto.
-    (* why does congruence not solve this? *)
-    assert (v0 = a0) by congruence; subst; auto.
   Qed.
 
   Theorem WaitForRead_ok : forall tid a,
       cprog_spec G tid
                  (fun v '(sigma_i, sigma) =>
                     {| precondition :=
-                         Sigma.disk sigma a = Some (v, Pending);
+                         Sigma.disk sigma a = Some (v, Pending) /\
+                         Sigma.l sigma = WriteLock;
                        postcondition :=
                          fun '(sigma_i', sigma') r =>
                            sigma_i' = sigma_i /\
@@ -49,19 +65,18 @@ Section Primitives.
   Proof.
     begin_prim.
     inv_bind; inv_exec.
+    inv_opt.
 
     eapply H2; eauto; simpl.
     intuition eauto.
-    (* why does congruence not solve this? *)
-    assert (v = a0) by congruence; subst; auto.
-    congruence.
   Qed.
 
   Theorem Write_ok : forall tid a v,
       cprog_spec G tid
                  (fun v0 '(sigma_i, sigma) =>
                     {| precondition :=
-                         Sigma.disk sigma a = Some (v0, NoReader);
+                         Sigma.disk sigma a = Some (v0, NoReader) /\
+                         Sigma.l sigma = WriteLock;
                        postcondition :=
                          fun '(sigma_i', sigma') _ =>
                            sigma_i' = sigma_i /\
@@ -70,15 +85,27 @@ Section Primitives.
   Proof.
     begin_prim.
     inv_bind; inv_exec.
+    inv_opt.
 
     eapply H2; eauto; simpl.
     intuition eauto.
   Qed.
 
+  Lemma read_permission_not_free : forall l,
+      ReadPermission l ->
+      l = Free ->
+      False.
+  Proof.
+    intros; subst.
+    inversion H.
+  Qed.
+
+  Hint Resolve read_permission_not_free.
+
   Theorem Get_ok : forall tid,
       cprog_spec G tid
                  (fun (_:unit) '(sigma_i, sigma) =>
-                    {| precondition := True;
+                    {| precondition := ReadPermission (Sigma.l sigma);
                        postcondition :=
                          fun  '(sigma_i', sigma') r =>
                            sigma_i' = sigma_i /\
@@ -87,7 +114,7 @@ Section Primitives.
                  Get.
   Proof.
     begin_prim.
-    inv_bind; inv_exec.
+    inv_bind; inv_exec; eauto.
 
     eapply H2; eauto; simpl.
     intuition eauto.
@@ -96,7 +123,7 @@ Section Primitives.
   Theorem Assgn_ok : forall tid m',
       cprog_spec G tid
                  (fun (_:unit) '(sigma_i, sigma) =>
-                    {| precondition := True;
+                    {| precondition := Sigma.l sigma = WriteLock;
                        postcondition :=
                          fun '(sigma_i', sigma') _ =>
                            sigma_i' = sigma_i /\
@@ -150,7 +177,7 @@ Section Primitives.
   Theorem GhostUpdate_ok : forall tid up,
       cprog_spec G tid
                  (fun (_:unit) '(sigma_i, sigma) =>
-                    {| precondition := True;
+                    {| precondition := Sigma.l sigma = WriteLock;
                        postcondition :=
                          fun '(sigma_i', sigma') _ =>
                            sigma_i' = sigma_i /\
@@ -164,23 +191,95 @@ Section Primitives.
     intuition eauto.
   Qed.
 
-  Theorem Yield_ok : forall tid,
+  Definition GetReadLock : @cprog St _ :=
+    SetLock ReadLock.
+
+  Definition GetWriteLock : @cprog St _ :=
+    SetLock WriteLock.
+
+  Definition ReleaseReadLock : @cprog St _ :=
+    SetLock Free.
+
+  Definition Unlock : @cprog St _ :=
+    SetLock Free.
+
+  Theorem GetReadLock_ok : forall tid,
       cprog_spec G tid
                  (fun (_:unit) '(sigma_i, sigma) =>
-                    {| precondition := G tid sigma_i sigma;
+                    {| precondition := Sigma.l sigma = Free;
                        postcondition :=
-                         fun '(sigma_i', sigma') _ =>
-                           Rely G tid sigma sigma' /\
-                           hashmap_le (Sigma.hm sigma) (Sigma.hm sigma') /\
-                           sigma_i' = sigma'; |})
-                 Yield.
+                         fun '(sigma_i', sigma'') _ =>
+                           exists sigma', Rely G tid sigma sigma' /\
+                                 sigma'' = Sigma.set_l sigma' ReadLock /\
+                                 hashmap_le (Sigma.hm sigma) (Sigma.hm sigma'') /\
+                                 sigma_i' = sigma''; |})
+                 GetReadLock.
   Proof.
     begin_prim.
     inv_bind; inv_exec.
 
-    eapply H2; eauto; simpl.
+    eapply H2; eauto.
     intuition eauto.
-    eauto.
+
+    eexists; intuition eauto.
+    destruct sigma'0; simpl; eauto.
+  Qed.
+
+  Theorem GetWriteLock_ok : forall tid,
+      cprog_spec G tid
+                 (fun (_:unit) '(sigma_i, sigma) =>
+                    {| precondition := Sigma.l sigma = Free;
+                       postcondition :=
+                         fun '(sigma_i', sigma'') _ =>
+                           exists sigma', Rely G tid sigma sigma' /\
+                                 sigma'' = Sigma.set_l sigma' WriteLock /\
+                                 hashmap_le (Sigma.hm sigma) (Sigma.hm sigma'') /\
+                                 sigma_i' = sigma''; |})
+                 GetWriteLock.
+  Proof.
+    begin_prim.
+    inv_bind; inv_exec.
+
+    eapply H2; eauto.
+    intuition eauto.
+
+    eexists; intuition eauto.
+    destruct sigma'0; simpl; eauto.
+  Qed.
+
+  Theorem ReleaseReadLock_ok : forall tid,
+      cprog_spec G tid
+                 (fun (_:unit) '(sigma_i, sigma) =>
+                    {| precondition := Sigma.l sigma = ReadLock;
+                       postcondition :=
+                         fun '(sigma_i', sigma') _ =>
+                           sigma' = Sigma.set_l sigma Free /\
+                           sigma_i' = sigma_i; |})
+                 ReleaseReadLock.
+  Proof.
+    begin_prim.
+    inv_bind; inv_exec.
+
+    eapply H2; eauto.
+    intuition eauto.
+  Qed.
+
+  Theorem Unlock_ok : forall tid,
+      cprog_spec G tid
+                 (fun (_:unit) '(sigma_i, sigma) =>
+                    {| precondition := Sigma.l sigma = WriteLock /\
+                                       G tid sigma_i sigma;
+                       postcondition :=
+                         fun '(sigma_i', sigma') _ =>
+                           sigma' = Sigma.set_l sigma Free /\
+                           sigma_i' = sigma'; |})
+                 Unlock.
+  Proof.
+    begin_prim.
+    inv_bind; inv_exec.
+
+    eapply H2; eauto.
+    intuition eauto.
   Qed.
 
 End Primitives.
@@ -193,7 +292,10 @@ Hint Extern 0 {{ Assgn _; _ }} => apply Assgn_ok : prog.
 Hint Extern 0 {{ Hash _; _ }} => apply Hash_ok : prog.
 Hint Extern 0 {{ Ret _; _ }} => apply Ret_ok : prog.
 Hint Extern 0 {{ GhostUpdate _; _ }} => apply GhostUpdate_ok : prog.
-Hint Extern 0 {{ @Yield _; _ }} => apply @Yield_ok : prog.
+Hint Extern 0 {{ GetReadLock; _ }} => apply GetReadLock_ok : prog.
+Hint Extern 0 {{ GetWriteLock; _ }} => apply GetWriteLock_ok : prog.
+Hint Extern 0 {{ ReleaseReadLock; _ }} => apply ReleaseReadLock_ok : prog.
+Hint Extern 0 {{ Unlock; _ }} => apply Unlock_ok : prog.
 
 (* Local Variables: *)
 (* company-coq-local-symbols: (("Sigma" . ?Σ) ("sigma" . ?σ) ("sigma'" . (?σ (Br . Bl) ?'))) *)
