src/CCLProg.v
@@ -17,30 +17,58 @@ Record StateTypes:Type :=
       Mem : Type;
       Abstraction : Type; }.
 
+Inductive LockState :=
+| Free
+| ReadLock
+| WriteLock.
+
+Inductive ReadPermission : LockState -> Prop :=
+| ReadPermissionR : ReadPermission ReadLock
+| ReadPermissionW : ReadPermission WriteLock.
+
+Definition CanRead (l:LockState) : {ReadPermission l} + {l = Free}.
+Proof.
+  destruct l; eauto using ReadPermissionR, ReadPermissionW.
+Qed.
+
+Definition CanWrite (l:LockState) : {l = WriteLock} + {l <> WriteLock}.
+Proof.
+  destruct l; left + right; congruence.
+Qed.
+
+Definition lock_dec (l l':LockState) : {l=l'}+{l<>l'}.
+Proof.
+  decide equality.
+Defined.
+
 (* The states a program steps through. *)
 Inductive Sigma St :=
-| state (d:DISK) (m:Mem St) (s:Abstraction St) (hm:hashmap).
+| state (d:DISK) (m:Mem St) (s:Abstraction St) (hm:hashmap) (l:LockState).
 
-Arguments state {St} d m s hm.
+Arguments state {St} d m s hm l.
 
 Module Sigma.
-  Definition disk St (s:Sigma St) :=
-    let (d, _, _, _) := s in d.
-  Definition mem St (s:Sigma St) :=
-    let (_, m, _, _) := s in m.
-  Definition s St (s:Sigma St) :=
-    let (_, _, s, _) := s in s.
-  Definition hm St (s:Sigma St) :=
-    let (_, _, _, hm) := s in hm.
+  Definition disk St (sigma:Sigma St) :=
+    let (d, _, _, _, _) := sigma in d.
+  Definition mem St (sigma:Sigma St) :=
+    let (_, m, _, _, _) := sigma in m.
+  Definition sigma St (sigma:Sigma St) :=
+    let (_, _, s, _, _) := sigma in s.
+  Definition hm St (sigma:Sigma St) :=
+    let (_, _, _, hm, _) := sigma in hm.
+  Definition l St (sigma:Sigma St) :=
+    let (_, _, _, _, l) := sigma in l.
 
-  Definition set_mem St (s:Sigma St) (m:Mem St) :=
-    let (d, _, s, hm) := s in state d m s hm.
-  Definition upd_disk St (s:Sigma St) (d':DISK -> DISK) :=
-    let (d, m, s, hm) := s in state (d' d) m s hm.
-  Definition upd_s St (s:Sigma St) (s':Abstraction St -> Abstraction St) :=
-    let (d, m, s, hm) := s in state d m (s' s) hm.
-  Definition upd_hm St (s:Sigma St) sz (buf: word sz) :=
-    let (d, m, s, hm) := s in state d m s (upd_hashmap' hm (hash_fwd buf) buf).
+  Definition set_mem St (sigma:Sigma St) (m:Mem St) :=
+    let (d, _, s, hm, l) := sigma in state d m s hm l.
+  Definition upd_disk St (sigma:Sigma St) (d':DISK -> DISK) :=
+    let (d, m, s, hm, l) := sigma in state (d' d) m s hm l.
+  Definition upd_s St (sigma:Sigma St) (s':Abstraction St -> Abstraction St) :=
+    let (d, m, s, hm, l) := sigma in state d m (s' s) hm l.
+  Definition upd_hm St (sigma:Sigma St) sz (buf: word sz) :=
+    let (d, m, s, hm, l) := sigma in state d m s (upd_hashmap' hm (hash_fwd buf) buf) l.
+  Definition set_l St (sigma:Sigma St) l :=
+    let (d, m, s, hm, _) := sigma in state d m s hm l.
 End Sigma.
 
 Section CCL.
@@ -59,62 +87,9 @@ Section CCL.
   | WaitForRead (a:addr) : cprog valu
   | Write (a:addr) (v: valu) : cprog unit
   | Hash sz (buf: word sz) : cprog (word hashlen)
-  | Yield : cprog unit
+  | SetLock (l:LockState) : cprog unit
   | Ret T (v:T) : cprog T
   | Bind T T' (p: cprog T') (p': T' -> cprog T) : cprog T.
-
-  Inductive step (tid:TID) (sigma: Sigma St) :
-    forall T, cprog T -> Sigma St -> T -> Prop :=
-  | StepGet :
-      step tid sigma Get sigma (Sigma.mem sigma)
-  | StepAssgn : forall m',
-      step tid sigma (Assgn m') (Sigma.set_mem sigma m') tt
-  | StepGhostUpdate : forall up,
-      step tid sigma (GhostUpdate up) (Sigma.upd_s sigma (up tid)) tt
-  | StepBeginRead : forall a v,
-      Sigma.disk sigma a = Some (v, NoReader) ->
-      step tid sigma (BeginRead a)
-           (Sigma.upd_disk sigma (fun d => upd d a (v, Pending))) tt
-  | StepWaitForRead : forall a v,
-      Sigma.disk sigma a = Some (v, Pending) ->
-      step tid sigma (WaitForRead a)
-           (Sigma.upd_disk sigma (fun d => upd d a (v, NoReader))) v
-  | StepWrite : forall a v0 v,
-      Sigma.disk sigma a = Some (v0, NoReader) ->
-      step tid sigma (Write a v)
-           (Sigma.upd_disk sigma (fun d => upd d a (v, NoReader))) tt
-  | StepHash : forall sz buf,
-      let h := hash_fwd buf in
-      hash_safe (Sigma.hm sigma) h buf ->
-      step tid sigma (@Hash sz buf)
-           (Sigma.upd_hm sigma buf) h.
-
-  Inductive fail_step (sigma: Sigma St) :
-    forall T, cprog T -> Prop :=
-  | FailStepBeginReadOob : forall a,
-      Sigma.disk sigma a = None ->
-      fail_step sigma (BeginRead a)
-  | FailStepBeginReadPending : forall a v,
-      Sigma.disk sigma a = Some (v, Pending) ->
-      fail_step sigma (BeginRead a)
-  | FailStepWaitForReadOob : forall a,
-      Sigma.disk sigma a = None ->
-      fail_step sigma (WaitForRead a)
-  | FailStepWaitForReadPending : forall a v,
-      Sigma.disk sigma a = Some (v, NoReader) ->
-      fail_step sigma (WaitForRead a)
-  | FailStepWriteOob : forall a v,
-      Sigma.disk sigma a = None ->
-      fail_step sigma (Write a v)
-  | FailStepWritePending : forall a v0 v,
-      Sigma.disk sigma a = Some (v0, Pending) ->
-      fail_step sigma (Write a v).
-
-  Inductive outcome T :=
-  | Finished (sigma_i sigma:Sigma St) (r:T)
-  | Error.
-
-  Arguments Error {T}.
 
   Definition Protocol := TID -> Sigma St -> Sigma St -> Prop.
   Variable Guarantee : Protocol.
@@ -125,14 +100,70 @@ Section CCL.
                            exists tid', tid <> tid' /\
                                    Guarantee tid sigma sigma').
 
+  Inductive StepOutcome T :=
+  | StepTo (sigma':Sigma St) (v:T)
+  | Fails
+  | NonDet.
+
+  Arguments Fails {T}.
+  Arguments NonDet {T}.
+
+  Definition step_dec tid (sigma: Sigma St) T (p: cprog T) : StepOutcome T :=
+    match p with
+    | Get => if CanRead (Sigma.l sigma) then StepTo sigma (Sigma.mem sigma)
+            else Fails
+    | Assgn m' => if CanWrite (Sigma.l sigma) then StepTo (Sigma.set_mem sigma m') tt
+                  else Fails
+    | GhostUpdate up => if CanWrite (Sigma.l sigma) then StepTo (Sigma.upd_s sigma (up tid)) tt
+                       else Fails
+    | BeginRead a => if CanWrite (Sigma.l sigma) then
+                      match Sigma.disk sigma a with
+                      | Some (v, NoReader) =>
+                        StepTo (Sigma.upd_disk sigma (fun d => upd d a (v, Pending))) tt
+                      | _ => Fails
+                      end
+                    else Fails
+    | WaitForRead a => if CanWrite (Sigma.l sigma) then
+                        match Sigma.disk sigma a with
+                        | Some (v, Pending) =>
+                          StepTo (Sigma.upd_disk sigma (fun d => upd d a (v, NoReader))) v
+                        | _ => Fails
+                        end
+                      else Fails
+    | Write a v => if CanWrite (Sigma.l sigma) then
+                    match Sigma.disk sigma a with
+                    | Some (_, NoReader) =>
+                      StepTo (Sigma.upd_disk sigma (fun d => upd d a (v, NoReader))) tt
+                    | _ => Fails
+                    end
+                  else Fails
+    | SetLock l' => if lock_dec (Sigma.l sigma) ReadLock then
+                     if lock_dec l' Free then
+                       StepTo (Sigma.set_l sigma Free) tt
+                     else Fails
+                   else NonDet
+    | Ret v => StepTo sigma v
+    | _ => NonDet
+    end.
+
+  Inductive outcome T :=
+  | Finished (sigma_i sigma:Sigma St) (r:T)
+  | Error.
+
+  Arguments Error {T}.
+
   Inductive exec (tid:TID) : forall T, (Sigma St * Sigma St) -> cprog T -> outcome T -> Prop :=
-  | ExecRet : forall T (v:T) sigma_i sigma, exec tid (sigma_i, sigma) (Ret v) (Finished sigma_i sigma v)
-  | ExecStep : forall T (p: cprog T) sigma_i sigma sigma' v,
-      step tid sigma p sigma' v ->
+  | ExecStepDec : forall T (p: cprog T) sigma_i sigma sigma' v,
+      step_dec tid sigma p = StepTo sigma' v ->
       exec tid (sigma_i, sigma) p (Finished sigma_i sigma' v)
-  | ExecFail : forall T (p: cprog T) sigma_i sigma,
-      fail_step sigma p ->
+  | ExecStepDecFail : forall T (p: cprog T) sigma_i sigma,
+      step_dec tid sigma p = Fails ->
       exec tid (sigma_i, sigma) p Error
+  | ExecHash : forall sigma_i sigma sz buf,
+      let h := hash_fwd buf in
+      hash_safe (Sigma.hm sigma) h buf ->
+      exec tid (sigma_i, sigma) (@Hash sz buf) (Finished sigma_i
+                                                     (Sigma.upd_hm sigma buf) h)
   | ExecBindFinish : forall T T' (p: cprog T') (p': T' -> cprog T)
                        sigma_i sigma sigma_i' sigma' v out,
       exec tid (sigma_i, sigma) p (Finished sigma_i' sigma' v) ->
@@ -141,14 +172,29 @@ Section CCL.
   | ExecBindFail : forall T T' (p: cprog T') (p': T' -> cprog T) sigma_i sigma,
       exec tid (sigma_i, sigma) p Error ->
       exec tid (sigma_i, sigma) (Bind p p') Error
-  | ExecYield : forall sigma_i sigma sigma',
-      Guarantee tid sigma_i sigma ->
+  | ExecLock : forall sigma_i sigma l' sigma',
+      Sigma.l sigma = Free ->
       Rely tid sigma sigma' ->
       hashmap_le (Sigma.hm sigma) (Sigma.hm sigma') ->
-      exec tid (sigma_i, sigma) Yield (Finished sigma' sigma' tt)
-  | ExecYieldFail : forall sigma_i sigma,
+      let sigma' := Sigma.set_l sigma' l' in
+      exec tid (sigma_i, sigma) (SetLock l') (Finished sigma' sigma' tt)
+  | ExecRelease : forall sigma_i sigma,
+      Sigma.l sigma = WriteLock ->
+      Guarantee tid sigma_i sigma ->
+      let sigma' := Sigma.set_l sigma Free in
+      exec tid (sigma_i, sigma) (SetLock Free) (Finished sigma' sigma' tt)
+  | ExecReleaseFail : forall sigma_i sigma,
+      Sigma.l sigma = WriteLock ->
       ~Guarantee tid sigma_i sigma ->
-      exec tid (sigma_i, sigma) Yield Error.
+      exec tid (sigma_i, sigma) (SetLock Free) Error.
+
+  Theorem ExecRet : forall tid T (v:T) sigma_i sigma,
+      exec tid (sigma_i, sigma) (Ret v) (Finished sigma_i sigma v).
+  Proof.
+    intros.
+    eapply ExecStepDec.
+    auto.
+  Qed.
 
   Definition SpecDouble T :=
     (Sigma St * Sigma St) -> (Sigma St * Sigma St -> T -> Prop) -> Prop.
@@ -185,16 +231,18 @@ Arguments Protocol St : clear implicits.
 
 Module CCLTactics.
   Import Automation.
+
+  Ltac inv_step :=
+    match goal with
+    | [ H: step_dec _ _ _ = _ |- _ ] =>
+      simpl in H; inversion H; subst; clear H
+    end.
+
   Ltac inv_bind :=
     match goal with
     | [ H: exec _ _ _ (Bind _ _) _ |- _ ] =>
       inversion H; subst; repeat inj_pair2;
-      try match goal with
-          | [ H: step _ _ _ _ _ |- _ ] =>
-            solve [ inversion H ]
-          | [ H: fail_step _ _ |- _ ] =>
-            solve [ inversion H ]
-          end;
+      try solve [ inv_step ];
       clear H
     end.
 
@@ -203,10 +251,8 @@ Module CCLTactics.
     | [ H: exec _ _ _ (Ret _) _ |- _ ] =>
       inversion H; subst; repeat inj_pair2;
       try match goal with
-          | [ H: step _ _ (Ret _) _ _ |- _ ] =>
-            solve [ inversion H ]
-          | [ H: fail_step _ (Ret _) |- _ ] =>
-            solve [ inversion H ]
+          | [ H: step_dec _ _ (Ret _) = _ |- _ ] =>
+            simpl in H; inversion H; subst; clear H
           end;
       clear H
     end.
@@ -217,24 +263,24 @@ Module CCLTactics.
   Ltac inv_exec' H :=
     inv_cleanup H;
     try match goal with
-        | [ H: step _ _ _ _ _ |- _ ] => inv_cleanup H
-        | [ H: fail_step _ _ |- _ ] => inv_cleanup H
-        end; try congruence.
+        | [ H: step_dec _ _ _ = _ |- _ ] =>
+          simpl in H;
+          repeat match goal with
+                 | [ H: context[match ?d with _ => _ end] |- _ ] =>
+                   destruct d; try congruence;
+                   let n := numgoals in guard n <= 1
+                 end
+        end;
+    repeat match goal with
+           | [ H: StepTo _ _ = StepTo _ _ |- _ ] =>
+             inversion H; subst; clear H
+           end;
+    try congruence.
 
   Ltac inv_exec :=
     match goal with
     | [ H: exec _ _ _ _ (Finished _ _ _) |- _ ] => inv_exec' H
     | [ H: exec _ _ _ _ Error |- _ ] => inv_exec' H
-    end.
-
-  Ltac inv_step :=
-    match goal with
-    | [ H: step _ _ _ _ _ |- _ ] => inversion H; subst
-    end.
-
-  Ltac inv_fail_step :=
-    match goal with
-    | [ H: fail_step _ _ |- _ ] => inversion H; subst
     end.
 
 End CCLTactics.
